src/Order copia.dfy
@@ -1,0 +1,44 @@
+predicate IsPreorder<A>(le: (A, A) -> bool, s:set<A>)
+{
+  (forall a | a in s :: le(a, a)) &&
+  (forall a, b, c | a in s && b in s && c in s && le(a, b) && le(b, c) :: le(a, c))
+}
+
+predicate IsTotalPreorder<A(!new)>(le: (A, A) -> bool)
+{
+  IsPreorder(le) &&
+  (forall a, b :: le(a, b) || le(b, a))
+}
+
+predicate IsPartialOrder<A(!new)>(le: (A, A) -> bool)
+{
+  (forall a :: le(a, a)) &&
+  (forall a, b | le(a, b) && le(b, a) :: a == b) &&
+  (forall a, b, c | le(a, b) && le(b, c) :: le(a, c))
+}
+
+predicate IsTotalOrder<A(!new)>(le: (A, A) -> bool)
+{
+  IsTotalPreorder(le) &&
+  (forall a, b | le(a, b) && le(b, a) :: a == b)
+}
+
+lemma PartialOrderAndTotalPreorder<A(!new)>(le: (A, A) -> bool)
+  requires IsTotalPreorder(le)
+  requires IsPartialOrder(le)
+  ensures IsTotalOrder(le)
+{
+}
+
+predicate Ordered<A>(xs: seq<A>, le: (A, A) -> bool)
+  requires IsTotalOrder(le)
+{
+  forall i, j | 0 <= i < j < |xs| :: le(xs[i], xs[j])
+}
+
+predicate OrderedInt(xs: seq<int>)
+{
+  //forall i, j | 0 <= i < j < |xs| :: xs[i] < xs[j]
+  Ordered<int>(xs,(x,y) => x<= y)
+}
+
